\section{Ableiten}

\subsection{Grundfunktionen}
\begin{itemize}
    \item $(a^x)' = a^x \cdot ln(x)$
    \item $(f(x)^{g(x)})' = f(x)^{g(x)} \cdot (ln(f(x)) \cdot g(x))'$
	\item $(x^r)' = r x^{r-1}$
	\item $(\frac{1}{x^r})' = \frac{r}{x^{r+1}}$
	\item $ln(x)' = \frac{1}{x}$
	\item $sin(x)' = cos(x)$
	\item $cos(x)' = -sin(x)$
	\item $arcsin(x)' = \frac{1}{\sqrt{1-x^2}}$
	\item $arccos(x)' = - \frac{1}{\sqrt{1-x^2}}$
	\item $arctan(x)' = \frac{1}{1-x^2}$

\end{itemize}

\subsection{Ableitungsregeln}
\begin{itemize}
	\item $f(x) = u(x) + v(x) \Rightarrow f'(x) = u'(x) + v'(x)$
	\item $f(x) = c u(x) \Rightarrow f'(x) = c u'(x)$
	\item $f(x) = u(x) v(x) \Rightarrow f'(x) = u'(x) v(x) + u(x) v'(x)$
	\item $f(x) = \frac{u(x)}{v(x)} \Rightarrow f'(x) = \frac{v(x) u'(x) - u(x) v'(x)}{v(x)^2}$
	\item $f(x) = u(v(x)) \Rightarrow f'(x) = u'(v(x)) v'(x)$
\end{itemize}
\subsubsection{Taylorreihe}
\begin{itemize}
	\item $T_a(f) = \sum_{i=0}^n \frac{f^{(i)}(a)}{i!}(x-a)^i$
\end{itemize}

\subsection{Trigonometrie}
\begin{itemize}
	\item $\alpha^\circ = \alpha^{(r)} \frac{180^\circ}{\pi}$
	\item $sin(\alpha)^2 + cos(\alpha)^2 = 1$
	\item $sin(-\alpha) = - sin(\alpha)$
	\item $cos(-\alpha) = cos(\alpha)$
	\item $sin(2\alpha) = 2 sin(\alpha) cos(\alpha)$
	\item $cos(2\alpha) = cos(\alpha)^2 - sin(\alpha)^2$
	\item $tan(\alpha) = \frac{sin(\alpha)}{cos(\alpha)}$
\end{itemize}

\subsection{Integrale}
\begin{itemize}
    \item $\int \frac{1}{x} = ln(x) + C$
    \item $\int ln(x) = -x + x ln(x) + C$
\end{itemize}

\subsection{Andere Formeln}
\begin{itemize}
    \item $i^2 = -1$
    \item $e^{i\varphi} = cos(\varphi) + i$
\end{itemize}
