\section{\lambda -Term Auswertung}

\subsection{Beispiele: Umgebung}
\begin{itemize}
    \item $(\lambda x.t) s \downarrow \phi$
    \begin{itemize}
        \item $s \downarrow \phi$
        \item $t \downarrow (s \leftarrow x) \circ \phi$
        \item $x \downarrow \phi = x$ falls $x \notin dom(\phi)$
    \end{itemize}

    \item $(\lambda x.t) \downarrow \phi = \lambda x.(t \downarrow \phi)$
    falls $x \notin \phi(y)$ f√ºr alle $y \in dom(y)$.

    \item $\lambda mnfx.mf(nfx)$ und $1 = \lambda gy.gy$
    \begin{enumerate}
        \item $((+ 1) 1) \downarrow \varepsilon$
        \item $1 \downarrow \varepsilon \rightarrow \lambda g.(\lambda y.gy) \downarrow \varepsilon$
        \item $\lambda g.(\lambda y.gy) \downarrow \varepsilon$
        \item $\lambda g.((\lambda y.gy) \downarrow \varepsilon)$
        \item $\lambda g.\lambda y.(gy \downarrow \varepsilon) = \lambda g.\lambda y.(g \downarrow \varepsilon)(y \downarrow \varepsilon) = 1$
        \item $(+ 1) \downarrow \varepsilon$
        \item $\lambda m.(\lambda nfx.mf(nfx)) 1 \downarrow \varepsilon$
        \item $\lambda nfx.(mf(nfx) \downarrow [1\leftarrow m] \circ \varepsilon)$
        \item $\lambda nfx.(m \downarrow [1\leftarrow m] \circ \varepsilon) f(nfx)$
        \item $\lambda nfx.1f(nfx)$
        \item $(+ 1) 1 \downarrow \varepsilon$
    \end{enumerate}
\end{itemize}
